cleaning up client logic and JSON structures for Resolute request/response, extracted and tested on microkit example

src/Resolute_Types.v
@@ -1,5 +1,4 @@
-Require Import Term_Defs Resolute_Logic JSON. (* Attestation_Session AppraisalSummary. *)
-(* Require Export Interface_Strings_Vars. *)
+Require Import Term_Defs Resolute_Logic JSON.
 
 Record Resolute_Client_Request := 
   mkResoluteClientReq {
@@ -9,22 +8,9 @@ Record Resolute_Client_Request :=
   }.
 
 Record Resolute_Client_Response := 
-  mkResoluteClientResp {
-    resclientresp_success: bool
-  }.
-
-Record Resolute_Client_Result := 
-  mkResoluteClientResult {
-    resclientres_term: Term;
-    resclientres_evidence: Evidence;
-    resclientres_success: bool;
-    resclientres_error_str: string;
-  }.
-
-
-Record ResoluteResponse := 
-    mkResoluteResp {
-      resoluteresp_judgement: Resolute_Judgement;
-      resoluteresp_formula: Resolute_Formula;
-      resoluteresp_term: Resolute_Term;
-  }.
+mkResoluteClientResp {
+  resclientres_term: Term;
+  resclientres_evidence: Evidence;
+  resclientres_success: bool;
+  resclientres_error_str: string;
+}.
