src/Concrete_Extractables.v
@@ -33,14 +33,6 @@ Definition concrete_Jsonifiable_ASP_ARGS : Jsonifiable ASP_ARGS.
 solve [typeclasses eauto].
 Defined.
 
-Definition concrete_Jsonifiable_ResoluteResponse : Jsonifiable ResoluteResponse.
-solve [typeclasses eauto].
-Defined.
-
 Definition concrete_Jsonifiable_Resolute_Client_Response : Jsonifiable Resolute_Client_Response.
-solve [typeclasses eauto].
-Defined.
-
-Definition concrete_Jsonifiable_Resolute_Client_Result : Jsonifiable Resolute_Client_Result.
 solve [typeclasses eauto].
 Defined.
